lean/src/r_correct_theorem.lean
@@ -1,7 +1,8 @@
 import tactic
 import .a_eval_theorem
-
 import .defs
+import .helper_defs
+
 variable [GuardModule]
 open GuardModule
 
@@ -21,7 +22,7 @@ begin
     simp [ant_eval, ant_eval_all, map_ant, ant_eval'],
 end
 
-lemma ant_eval_branch (tr1: Ant Φ) (tr2: Ant Φ) (env: Env) (r: Result)
+lemma ant_eval_branch { tr1: Ant Φ } { tr2: Ant Φ } { env: Env } { r: Result }
     (h: ant_eval (tr1.branch tr2) env = some r):
         ant_eval tr1 env = some r ∨ ant_eval tr2 env = some r :=
 begin
@@ -45,114 +46,95 @@ begin
     finish,
 end
 
-def ℛ'_diverge (a: list Leaf) (i: list Leaf) (r: list Leaf) (is_empty: bool) (ant: Ant bool)
-    (h1: ℛ' ant = (a, i, r)):
-    (is_empty = false ∧ a = [] ∧ i = []  ∧ ∃ rh: Leaf, ∃ rs: list Leaf, r = rh::rs ∧ ℛ' (Ant.diverge is_empty ant) = ([], [rh], rs))
-    ∨ ((is_empty = true ∨ a ≠ [] ∨ i ≠ [] ∨ r = []) ∧ ℛ' (Ant.diverge is_empty ant) = (a, i, r)) :=
+def R_diverge { is_empty: Φ → bool } { tr: Ant Φ } { r: LeafPartition } (ty: Φ)
+    (h: R is_empty tr = r):
+    (∃ rh: Leaf, ∃ rs: list Leaf, is_empty ty = ff ∧ r = ⟨ [], [], rh::rs ⟩ ∧ R is_empty (Ant.diverge ty tr) = ⟨ [], [rh], rs ⟩)
+    ∨ ((is_empty ty = tt ∨ r.acc ≠ [] ∨ r.inacc ≠ [] ∨ r.red = []) ∧ R is_empty (Ant.diverge ty tr) = r) :=
 begin
-    cases is_empty;
-    cases a;
-    cases i;
+    unfold R R' map_ant,
+    unfold R at h,
+    
+    cases is_empty ty;
     cases r;
-    simp [ℛ', ℛ'._match_1, h1],
+    cases r_acc;
+    cases r_inacc;
+    cases r_red;
+    simp [h, R'._match_1],
+end
+
+@[simp]
+lemma is_empty_implies_eval_false { is_empty: Gs } { ty: Φ} { env: Env} (h: is_empty.val ty = tt): Φ_eval ty env = ff :=
+begin
+    have := is_empty.property,
+    finish [is_empty_prover],
+end
+
+@[simp]
+lemma eval_true_imples_empty_false (is_empty: Gs) { ty: Φ } { env: Env } (h: Φ_eval ty env = tt): is_empty.val ty = ff :=
+begin
+    by_contra,
+    have := is_empty.property,
+    finish [is_empty_prover],
 end
 
 -- (a, i, r) = ℛ is_empty.val (Ant.diverge ant_a ant_tr)
-
-def ℛ'_diverge' (ty: Φ) (tr: Ant Φ) (): sorry := sorry
+attribute [simp] R map_ant R'
+local attribute [simp] ant_eval ant_eval' ant_eval_all
 
 lemma r_correct_1 [decidable_eq Leaf]
     (is_empty: Gs) (gdt: Gdt)
     
     (ant: Ant Φ)
-    (h1: ant_eval ant = some ∘ gdt_eval gdt)
-
-    (a: list Leaf) (i: list Leaf) (r: list Leaf)
-    (h2: (a, i, r) = ℛ is_empty.val ant)
+    (h_ant: ant_eval ant = some ∘ gdt_eval gdt)
     
     (env: Env) (leaf: Leaf)
-    (h3: gdt_eval gdt env = Result.leaf leaf):
+    (h_leaf: gdt_eval gdt env = Result.leaf leaf):
 
-        leaf ∈ a
+        leaf ∈ (R is_empty.val ant).acc
 
     :=
 begin
-    replace h3: ant_eval ant env = some(Result.leaf leaf), sorry, -- finish
-    clear h1,
+    have h: ant_eval ant env = some(Result.leaf leaf), simp [h_ant, h_leaf],
+    clear h_ant h_leaf,
     
-    induction ant generalizing a i r env,
+    induction ant generalizing  env,
 
+    case Ant.leaf {       
+        cases c: Φ_eval ant_a env,
+        {
+            finish,
+        },
+        {
+            have:= eval_true_imples_empty_false is_empty c,
+            finish,
+        }
+    },
     case Ant.branch {
-        sorry,
-        /-
-        rw ℛ at h2,
-        rw map_ant at h2,
-        rw ℛ' at h2,
-        rw ←ℛ at h2,
-        rw ←ℛ at h2,
-
-        replace h3 := ant_eval_branch h3,
-
-        cases ℛ is_empty.val ant_tr1 with tr1_a tr1_,
-        cases tr1_ with tr1_i tr1_r,
-
-        cases ℛ is_empty.val ant_tr2 with tr2_a tr2_,
-        cases tr2_ with tr2_i tr2_r,
-
-
-        rw ℛ'._match_2 at h2,
-
-        cases h3,
-
+        replace h := ant_eval_branch h,
+        cases h,
         case or.inl {
-            have: leaf ∈ tr1_a := begin
-                specialize ant_ih_tr1 tr1_a tr1_i tr1_r env,
-                simp at ant_ih_tr1,
-                rw h3 at ant_ih_tr1,
-                simp at ant_ih_tr1,
-                exact ant_ih_tr1,
-            end,
+            specialize ant_ih_tr1 env h,
             finish,
         },
-
         case or.inr {
-            have: leaf ∈ tr2_a := begin
-                specialize ant_ih_tr2 tr2_a tr2_i tr2_r env,
-                simp at ant_ih_tr2,
-                rw h3 at ant_ih_tr2,
-                simp at ant_ih_tr2,
-                exact ant_ih_tr2,
-            end,
+            specialize ant_ih_tr2 env h,
+            finish,
+        }
+    },
+    case Ant.diverge {
+        replace h := ant_eval_diverge h,
+        let r := R is_empty.val ant_tr,
+        have y := R_diverge ant_a (refl r),
+        
+        cases y,
+        {
+            cases y with rh y,
+            cases y with rs y,
             finish,
         },
-        -/
-    },
-
-    case Ant.diverge {
-        rw ℛ at h2,
-        rw map_ant at h2,
-        rw ℛ' at h2,
-        rw ←ℛ at h2,
-
-        replace h3 := ant_eval_diverge h3,
-        cases ℛ is_empty.val ant_tr with tr_a tr_,
-        cases tr_ with tr_i tr_r,
-
-        have x := ℛ'_diverge a i r (is_empty.val ant_a) (map_ant is_empty.val ant_tr),
-        rw ℛ at h2,
-        rw h2 at x,
-
-        rw ℛ'._match_1 at h2,
-    },
+        finish,
+    }
 end
-
-
-#print prefix ℛ'._match_1
-
-
-
-
-
 
 
 
